src/Init/Data/Iterators/Lemmas/Consumers/Loop.lean
@@ -6,8 +6,8 @@ Authors: Paul Reichert
 prelude
 import Init.Data.List.Control
 import Std.Data.Iterators.Lemmas.Basic
-import Std.Data.Iterators.Lemmas.Consumers.Collect
-import Std.Data.Iterators.Lemmas.Consumers.Monadic.Loop
+import Init.Data.Iterators.Lemmas.Consumers.Collect
+import Init.Data.Iterators.Lemmas.Consumers.Monadic.Loop
 import Init.Data.Iterators.Consumers.Collect
 import Init.Data.Iterators.Consumers.Loop
 
