src/Init/Data/Iterators/Lemmas/Consumers/Monadic/Loop.lean
@@ -8,7 +8,7 @@ import Init.Control.Lawful.Basic
 import Init.Data.Iterators.Consumers.Monadic.Collect
 import Init.Data.Iterators.Consumers.Monadic.Loop
 import Std.Data.Iterators.Lemmas.Monadic.Basic
-import Std.Data.Iterators.Lemmas.Consumers.Monadic.Collect
+import Init.Data.Iterators.Lemmas.Consumers.Monadic.Collect
 import Std.Data.Iterators.Lemmas.Equivalence.StepCongr
 
 namespace Std.Iterators
