src/Init/Data/Range/New/Lemmas.lean
@@ -2,90 +2,117 @@ module
 
 prelude
 import all Init.Data.Range.New.Nat
+import Init.Data.List.Range
 
 namespace Std.PRange
 
-/-- Generalization of `mem_of_mem_range'` used in `forIn'_loop_eq_forIn'_range'` below. -/
-private theorem mem_of_mem_range'_aux {r : Range} {a : Nat} (w₁ : (i - r.start) % r.step = 0)
-    (w₂ : r.start ≤ i)
-    (h : a ∈ List.range' i ((r.stop - i + r.step - 1) / r.step) r.step) : a ∈ r := by
-  obtain ⟨j, h', rfl⟩ := List.mem_range'.1 h
-  refine ⟨by omega, ?_⟩
-  rw [Nat.lt_div_iff_mul_lt r.step_pos, Nat.mul_comm] at h'
-  constructor
-  · omega
-  · rwa [Nat.add_comm, Nat.add_sub_assoc w₂, Nat.mul_add_mod_self_left]
+-- /-- Generalization of `mem_of_mem_range'` used in `forIn'_loop_eq_forIn'_range'` below. -/
+-- private theorem mem_of_mem_range'_aux [LE α] {r : PRange ⟨.closed, .closed⟩ α} {a : α}
+--     -- (w₁ : (i - r.lower) % r.step = 0)
+--     (w₂ : r.lower ≤ i)
+--     (h : a ∈ List.polymorphicRange i ((r.upper - i + r.step - 1) / r.step) r.step) : a ∈ r := by
+--   obtain ⟨j, h', rfl⟩ := List.mem_range'.1 h
+--   refine ⟨by omega, ?_⟩
+--   rw [Nat.lt_div_iff_mul_lt r.step_pos, Nat.mul_comm] at h'
+--   constructor
+--   · omega
+--   · rwa [Nat.add_comm, Nat.add_sub_assoc w₂, Nat.mul_add_mod_self_left]
 
-theorem mem_of_mem_range' {r : Range} (h : x ∈ List.range' r.start r.size r.step) : x ∈ r := by
-  unfold size at h
-  apply mem_of_mem_range'_aux (by simp) (by simp) h
+-- theorem mem_of_mem_range' [Succ? α] [LE α] [DecidableLE α] {r : PRange ⟨.closed, .closed⟩ α}
+--     [LawfulSucc? α]
+--     (h : x ∈ List.polymorphicRange r.lower r.size 1) : x ∈ r := by
+--   refine ⟨?_, ?_⟩
+--   ·
+--   unfold PRange.size at h
+--   apply mem_of_mem_range'_aux (by simp) (by simp) h
 
-private theorem size_eq (r : Std.Range) (h : i < r.stop) :
-    (r.stop - i + r.step - 1) / r.step =
-      (r.stop - (i + r.step) + r.step - 1) / r.step + 1 := by
-  have w := r.step_pos
-  if i + r.step < r.stop then -- Not sure this case split is strictly necessary.
-    rw [Nat.div_eq_iff w, Nat.add_one_mul]
-    have : (r.stop - (i + r.step) + r.step - 1) / r.step * r.step ≤
-        (r.stop - (i + r.step) + r.step - 1) := Nat.div_mul_le_self _ _
-    have : r.stop - (i + r.step) + r.step - 1 - r.step <
-        (r.stop - (i + r.step) + r.step - 1) / r.step * r.step :=
-      Nat.lt_div_mul_self w (by omega)
-    omega
-  else
-    have : (r.stop - i + r.step - 1) / r.step = 1 := by
-      rw [Nat.div_eq_iff w, Nat.one_mul]
-      omega
-    have : (r.stop - (i + r.step) + r.step - 1) / r.step = 0 := by
-      rw [Nat.div_eq_iff] <;> omega
-    omega
+@[simp] theorem mem_of_mem_toList [Succ? α] [LE α] [DecidableLE α]
+    [LawfulLESucc? α] [Monad m]
+    (r : PRange ⟨.closed, .closed⟩ α)
+    (h : a ∈ r.toList) :
+    a ∈ r := by
+  refine ⟨?_, ?_⟩
+  · sorry -- a is an indirect output
+    -- hence, a has been obtained from a chain of `succ?`
+    -- hence, a is large enough
+  · sorry -- a is an indirect output, hence small enough
 
-private theorem forIn'_loop_eq_forIn'_range' [Monad m] (r : Std.Range)
-    (init : β) (f : (a : Nat) → a ∈ r → β → m (ForInStep β)) (i) (w₁) (w₂) :
-    forIn'.loop r f init i w₁ w₂ =
-      forIn' (List.range' i ((r.stop - i + r.step - 1) / r.step) r.step) init
-        fun a h => f a (mem_of_mem_range'_aux w₁ w₂ h) := by
-  have w := r.step_pos
-  rw [forIn'.loop]
-  split <;> rename_i h
-  · simp only [size_eq r h, List.range'_succ, List.forIn'_cons]
-    congr 1
-    funext step
-    split
-    · simp
-    · rw [forIn'_loop_eq_forIn'_range']
-  · have : (r.stop - i + r.step - 1) / r.step = 0 := by
-      rw [Nat.div_eq_iff] <;> omega
-    simp [this]
+-- @[simp] theorem forIn'_eq_forIn'_toList [Succ? α] [LE α] [DecidableLE α]
+--     [LawfulLESucc? α] [Monad m]
+--     (r : PRange ⟨.closed, .closed⟩ α)
+--     (init : β) (f : (a : α) → a ∈ r → β → m (ForInStep β)) :
+--     forIn' r init f =
+--       forIn' r.toList init (fun a h => f a sorry) := by
+--   conv => lhs; simp only [forIn', Range.forIn']
+--   simp only [size]
+--   rw [forIn'_loop_eq_forIn'_range']
 
-@[simp] theorem forIn'_eq_forIn'_range' [Monad m] (r : Std.Range)
-    (init : β) (f : (a : Nat) → a ∈ r → β → m (ForInStep β)) :
-    forIn' r init f =
-      forIn' (List.range' r.start r.size r.step) init (fun a h => f a (mem_of_mem_range' h)) := by
-  conv => lhs; simp only [forIn', Range.forIn']
-  simp only [size]
-  rw [forIn'_loop_eq_forIn'_range']
+-- private theorem size_eq (r : Std.Range) (h : i < r.stop) :
+--     (r.stop - i + r.step - 1) / r.step =
+--       (r.stop - (i + r.step) + r.step - 1) / r.step + 1 := by
+--   have w := r.step_pos
+--   if i + r.step < r.stop then -- Not sure this case split is strictly necessary.
+--     rw [Nat.div_eq_iff w, Nat.add_one_mul]
+--     have : (r.stop - (i + r.step) + r.step - 1) / r.step * r.step ≤
+--         (r.stop - (i + r.step) + r.step - 1) := Nat.div_mul_le_self _ _
+--     have : r.stop - (i + r.step) + r.step - 1 - r.step <
+--         (r.stop - (i + r.step) + r.step - 1) / r.step * r.step :=
+--       Nat.lt_div_mul_self w (by omega)
+--     omega
+--   else
+--     have : (r.stop - i + r.step - 1) / r.step = 1 := by
+--       rw [Nat.div_eq_iff w, Nat.one_mul]
+--       omega
+--     have : (r.stop - (i + r.step) + r.step - 1) / r.step = 0 := by
+--       rw [Nat.div_eq_iff] <;> omega
+--     omega
 
-@[simp] theorem forIn_eq_forIn_range' [Monad m] (r : Std.Range)
-    (init : β) (f : Nat → β → m (ForInStep β)) :
-    forIn r init f = forIn (List.range' r.start r.size r.step) init f := by
-  simp only [forIn, forIn'_eq_forIn'_range']
+-- private theorem forIn'_loop_eq_forIn'_range' [Monad m] (r : Std.Range)
+--     (init : β) (f : (a : Nat) → a ∈ r → β → m (ForInStep β)) (i) (w₁) (w₂) :
+--     forIn'.loop r f init i w₁ w₂ =
+--       forIn' (List.range' i ((r.stop - i + r.step - 1) / r.step) r.step) init
+--         fun a h => f a (mem_of_mem_range'_aux w₁ w₂ h) := by
+--   have w := r.step_pos
+--   rw [forIn'.loop]
+--   split <;> rename_i h
+--   · simp only [size_eq r h, List.range'_succ, List.forIn'_cons]
+--     congr 1
+--     funext step
+--     split
+--     · simp
+--     · rw [forIn'_loop_eq_forIn'_range']
+--   · have : (r.stop - i + r.step - 1) / r.step = 0 := by
+--       rw [Nat.div_eq_iff] <;> omega
+--     simp [this]
 
-private theorem forM_loop_eq_forM_range' [Monad m] (r : Std.Range) (f : Nat → m PUnit) :
-    forM.loop r f i = forM (List.range' i ((r.stop - i + r.step - 1) / r.step) r.step) f := by
-  have w := r.step_pos
-  rw [forM.loop]
-  split <;> rename_i h
-  · simp [size_eq r h, List.range'_succ, List.forM_cons]
-    congr 1
-    funext
-    rw [forM_loop_eq_forM_range']
-  · have : (r.stop - i + r.step - 1) / r.step = 0 := by
-      rw [Nat.div_eq_iff] <;> omega
-    simp [this]
+-- @[simp] theorem forIn'_eq_forIn'_range' [Monad m] (r : Std.Range)
+--     (init : β) (f : (a : Nat) → a ∈ r → β → m (ForInStep β)) :
+--     forIn' r init f =
+--       forIn' (List.range' r.start r.size r.step) init (fun a h => f a (mem_of_mem_range' h)) := by
+--   conv => lhs; simp only [forIn', Range.forIn']
+--   simp only [size]
+--   rw [forIn'_loop_eq_forIn'_range']
 
-@[simp] theorem forM_eq_forM_range' [Monad m] (r : Std.Range) (f : Nat → m PUnit) :
-    forM r f = forM (List.range' r.start r.size r.step) f := by
-  simp only [forM, Range.forM, forM_loop_eq_forM_range', size]
+-- @[simp] theorem forIn_eq_forIn_range' [Monad m] (r : Std.Range)
+--     (init : β) (f : Nat → β → m (ForInStep β)) :
+--     forIn r init f = forIn (List.range' r.start r.size r.step) init f := by
+--   simp only [forIn, forIn'_eq_forIn'_range']
 
-end Std.Range
+-- private theorem forM_loop_eq_forM_range' [Monad m] (r : Std.Range) (f : Nat → m PUnit) :
+--     forM.loop r f i = forM (List.range' i ((r.stop - i + r.step - 1) / r.step) r.step) f := by
+--   have w := r.step_pos
+--   rw [forM.loop]
+--   split <;> rename_i h
+--   · simp [size_eq r h, List.range'_succ, List.forM_cons]
+--     congr 1
+--     funext
+--     rw [forM_loop_eq_forM_range']
+--   · have : (r.stop - i + r.step - 1) / r.step = 0 := by
+--       rw [Nat.div_eq_iff] <;> omega
+--     simp [this]
+
+-- @[simp] theorem forM_eq_forM_range' [Monad m] (r : Std.Range) (f : Nat → m PUnit) :
+--     forM r f = forM (List.range' r.start r.size r.step) f := by
+--   simp only [forM, Range.forM, forM_loop_eq_forM_range', size]
+
+-- end Std.Range
