src/Init/Data/Range/New/Nat.lean
@@ -2,31 +2,31 @@ module
 
 prelude
 import all Init.Data.Range.New.Basic
-import Init.Omega
 
 open Std.Iterators
 
-instance : Succ? Nat where
-  succ? n := some (n + 1)
-  succAtIdx? k n := some (n + k)
+-- instance : Succ? Nat where
+--   succ? n := some (n + 1)
+--   succAtIdx? k n := some (n + k)
 
-instance : LawfulLESucc? Nat where
-  le_rfl := Nat.le_refl _
-  le_succ?_of_le hle h := by
-    simp only [Succ?.succ?, Option.some.injEq] at h
-    omega
-  le_succAtIdx?_of_le {a b c n} hle h := by
-    simp only [Succ?.succAtIdx?, Option.some.injEq] at h
-    omega
-    -- simp only [Succ?.succAtIdx?, Option.bind_eq_bind] at h
-    -- induction n generalizing b c with
-    -- | zero => simp_all [Nat.repeat]
-    -- | succ n ih =>
-    --   simp only [Nat.repeat, Option.bind_eq_some_iff] at h ih
-    --   rcases h with ⟨c', hc', h⟩
-    --   cases h
-    --   specialize ih hle hc'
-    --   omega
+-- instance : LawfulLESucc? Nat where
+--   le_rfl := Nat.le_refl _
+--   le_succ? := sorry
+--   le_succ?_of_le hle h := by
+--     simp only [Succ?.succ?, Option.some.injEq] at h
+--     sorry
+--   le_succAtIdx?_of_le {a b c n} hle h := by
+--     simp only [Succ?.succAtIdx?, Option.some.injEq] at h
+--     sorry
+--     -- simp only [Succ?.succAtIdx?, Option.bind_eq_bind] at h
+--     -- induction n generalizing b c with
+--     -- | zero => simp_all [Nat.repeat]
+--     -- | succ n ih =>
+--     --   simp only [Nat.repeat, Option.bind_eq_some_iff] at h ih
+--     --   rcases h with ⟨c', hc', h⟩
+--     --   cases h
+--     --   specialize ih hle hc'
+--     --   omega
 
 -- instance (stepSize : Nat) (h) :
 --     Finite (Range.SuccIterator (α := Nat) stepSize (· ≤ n) h) Id := by
