src/Std/Data/Iterators/Lemmas/Combinators/TakeWhile.lean
@@ -6,7 +6,7 @@ Authors: Paul Reichert
 prelude
 import Std.Data.Iterators.Combinators.TakeWhile
 import Std.Data.Iterators.Lemmas.Combinators.Monadic.TakeWhile
-import Std.Data.Iterators.Lemmas.Consumers
+import Init.Data.Iterators.Lemmas.Consumers
 
 namespace Std.Iterators
 
